Introduce Iterator for TreeParser and prove TreeParser terminates

Validator/Capturer/Inst/TreeParserLogCaptureM.lean
@@ -8,12 +8,12 @@ import Validator.Capturer.CaptureM
 namespace TreeParserLogCaptureM
 
 structure State (α: Type) where
-  parser: TreeParser.TreeParser α
+  parser: TreeParser.ParserState α
   logs : List String
 
 abbrev Impl α β := EStateM String (State α) β
 
-def Impl.mk (p: TreeParser.TreeParser α): State α :=
+def Impl.mk (p: TreeParser.ParserState α): State α :=
   State.mk p []
 
 instance : Debug (Impl α) where
@@ -22,15 +22,15 @@ instance : Debug (Impl α) where
     set (State.mk s.parser (s.logs ++ [line]))
     return ()
 
-instance: MonadStateOf (TreeParser.TreeParser α) (Impl α) where
-  get : Impl α (TreeParser.TreeParser α) := do
+instance: MonadStateOf (TreeParser.ParserState α) (Impl α) where
+  get : Impl α (TreeParser.ParserState α) := do
     let s <- EStateM.get
     return s.parser
-  set : TreeParser.TreeParser α → Impl α PUnit :=
+  set : TreeParser.ParserState α → Impl α PUnit :=
     fun parser => do
       let s <- EStateM.get
       EStateM.set (State.mk parser s.logs)
-  modifyGet {β: Type}: (TreeParser.TreeParser α → Prod β (TreeParser.TreeParser α)) → Impl α β :=
+  modifyGet {β: Type}: (TreeParser.ParserState α → Prod β (TreeParser.ParserState α)) → Impl α β :=
     fun f => do
       let s <- EStateM.get
       let (res, parser) := f s.parser
@@ -41,7 +41,7 @@ instance
   [Monad (Impl α)] -- EStateM is monad
   [Debug (Impl α)] -- Debug instance is declared above
   [MonadExcept String (Impl α)] -- EStateM String is MonadExcept String
-  [MonadStateOf (TreeParser.TreeParser α) (Impl α)] -- MonadStateOf ParseTree.TreeParser is declared above
+  [MonadStateOf (TreeParser.ParserState α) (Impl α)] -- MonadStateOf ParseTree.TreeParser is declared above
   : Parser (Impl α) α where -- This should just follow, but apparently we need to spell it out
   next := Parser.next
   skip := Parser.skip
@@ -51,9 +51,9 @@ instance : CaptureM (Impl α) α where
   -- all instances have been created, so no implementations are required here
 
 def run (f: Impl α β) (forest: ParseForest α): EStateM.Result String (State α) β :=
-  EStateM.run f (Impl.mk (TreeParser.TreeParser.mks forest))
+  EStateM.run f (Impl.mk (TreeParser.ParserState.mks forest))
 
 def run' (f: Impl α β) (forest: ParseForest α): (List String × (Except String β)) :=
-  match EStateM.run f (Impl.mk (TreeParser.TreeParser.mks forest)) with
+  match EStateM.run f (Impl.mk (TreeParser.ParserState.mks forest)) with
   | EStateM.Result.ok res s => (s.logs, Except.ok res)
   | EStateM.Result.error err s => (s.logs, Except.error err)
