Validator/Parser/Stack.lean
@@ -1,32 +1,40 @@
-inductive Stack (α: Type u) where
-  | mk (current: α) (stack: List α)
+abbrev Stack α := List α
 
 namespace Stack
 
-def getCurrent {α: outParam Type} [Monad m] [MonadState (Stack α) m]: m α := do
-  let s <- get
-  match s with
-  | Stack.mk curr _ => return curr
+def getCurrent? {α: outParam Type} (stack: Stack α) : Option α :=
+  match stack with
+  | [] => Option.none
+  | curr::_ => curr
 
-def setCurrent [Monad m] [MonadStateOf (Stack α) m] (t: α): m Unit := do
-  let s <- get
-  match s with
-  | Stack.mk _ stack =>
-    set (Stack.mk t stack)
+def isEmpty (stack: Stack α): Bool :=
+  match stack with
+  | [] => true
+  | _ => false
+
+def getCurrentM? {α: outParam Type} [Monad m] [MonadState (Stack α) m]: m (Option α) := do
+  let stack <- get
+  return stack.getCurrent?
+
+def setCurrentM [Monad m] [MonadExcept String m] [MonadStateOf (Stack α) m] (current: α): m Unit := do
+  let stack <- get
+  match stack with
+  | [] =>
+    throw "cannot setCurrent, stack is empty"
+  | _::rest =>
+    set (current::rest)
     return ()
 
-def push [Monad m] [MonadStateOf (Stack α) m] (top: α): m Unit := do
-  let s <- get
-  match s with
-  | Stack.mk oldtop stack =>
-    set (Stack.mk top (oldtop::stack))
-    return ()
+def pushM [Monad m] [MonadStateOf (Stack α) m] (top: α): m Unit := do
+  let stack <- get
+  set (top::stack)
+  return ()
 
-def pop [Monad m] [MonadStateOf (Stack α) m]: m Bool := do
-  let s <- get
-  match s with
-  | Stack.mk _ [] =>
-    return false
-  | Stack.mk _ (newtop::stack) =>
-    set (Stack.mk newtop stack)
-    return true
+def popM? [Monad m] [MonadStateOf (Stack α) m]: m (Option α) := do
+  let stack <- get
+  match stack with
+  | [] =>
+    return Option.none
+  | top::rest =>
+    set rest
+    return Option.some top
