Validator/Parser/TreeParser.lean
@@ -1,3 +1,4 @@
+import Validator.Std.Ltac
 import Validator.Std.Debug
 import Validator.Std.Except
 
@@ -7,9 +8,32 @@ import Validator.Parser.Stack
 import Validator.Parser.ParseTree
 import Validator.Parser.Parser
 
+local elab "simp_monads" : tactic => do
+  run `(tactic| simp [
+    getThe,
+    Bind.bind,
+    Except.bind,
+    Except.map,
+    Except.pure,
+    Functor.map,
+    MonadState.get,
+    MonadStateOf.get,
+    MonadStateOf.set,
+    Pure.pure,
+    StateT.bind,
+    StateT.get,
+    StateT.map,
+    StateT.pure,
+    StateT.run,
+    StateT.set] )
+
 namespace TreeParser
 
-inductive ParserState (α: Type) where
+open Nat
+
+abbrev ParseStack α := Stack (ParseForest α)
+
+inductive CurrentState (α: Type) where
   | unknown (children: ParseForest α)
   | opened (nexts: ParseForest α)
   | value (v: α) (nexts: ParseForest α)
@@ -17,194 +41,664 @@ inductive ParserState (α: Type) where
   | field (f: α) (children: ParseForest α)
   | eof
 
-abbrev TreeParser α := Stack (ParserState α)
+structure ParserState α where
+  current: CurrentState α
+  stack: ParseStack α
 
-def TreeParser.pop [Monad m] [MonadStateOf (TreeParser α) m]: m Bool :=
-  Stack.pop (α := ParserState α)
+def ParserState.mk' (tree: ParseTree α): ParserState α :=
+  ParserState.mk (CurrentState.unknown [tree]) []
 
-def TreeParser.mk (tree: ParseTree α): TreeParser α :=
-  Stack.mk (ParserState.unknown [tree]) []
+def ParserState.mks (forest: ParseForest α): ParserState α :=
+  ParserState.mk (CurrentState.unknown forest) []
 
-def TreeParser.mks (forest: ParseForest α): TreeParser α :=
-  Stack.mk (ParserState.unknown forest) []
+mutual
+@[simp]
+noncomputable def ParseTree.size (x: ParseTree α): Nat :=
+  match x with
+  | ParseTree.mk _ children =>
+    1 + ParseForest.size children
+@[simp]
+noncomputable def ParseForest.size (xs: ParseForest α): Nat :=
+  match xs with
+  | [] => 1
+  | (x::xs') => 1 + ParseTree.size x + ParseForest.size xs'
+end
+
+@[simp]
+noncomputable def ParseStack.size (s: ParseStack α): Nat :=
+  match s with
+  | [] => 0
+  | (x::xs) => ParseForest.size x + ParseStack.size xs
+
+@[simp]
+noncomputable def CurrentState.size (s: CurrentState α): Nat :=
+  match s with
+  -- unknown needs to be the larger than opened, since it is the next state.
+  | CurrentState.unknown forest => 4 + ParseForest.size forest
+  -- field needs to be larger than opened, since opened follows from field.
+  | CurrentState.field _ forest => 3 + ParseForest.size forest
+  -- pair can only be one smaller than opened
+  | CurrentState.pair _ _ forest => 3 + ParseForest.size forest
+  -- opened is always the second state, but also follows from field, so it needs to be smaller than unknown and field.
+  | CurrentState.opened forest => 2 + ParseForest.size forest
+  -- value needs to smaller than pair and smaller or equal to opened
+  | CurrentState.value _ forest => 2 + ParseForest.size forest
+  -- eof
+  | CurrentState.eof => 0
+
+-- When calling next, none of the states grow the stack, except for:
+-- ParserState.opened (t::nexts) and ParserState.value _ (t::nexts)
+--   where t = ParseTree.mk f children
+--         children ≠ []
+--         children ≠ [ParseTree.mk v []]
+-- These result in two states:
+--   Stack.setCurrentM (ParserState.opened nexts)
+--   Stack.pushM (ParserState.field f children)
+-- We need to make sure that these two states together are smaller than the previous state.
+-- This implies that we need show that the stack gets smaller as it grows in these two cases:
+--   theorem sizeOf_opened_gt_push: ParserState.opened (t::nexts)  > ParserState.opened nexts + ParserState.field f children
+--   theorem sizeOf_value_gt_push: ParserState.value _ (t::nexts) > ParserState.opened nexts + ParserState.field f children
+-- While also making sure that as the stack shrinks for these two cases that it also gets smaller:
+--   theorem sizeOf_value_gt_popped_value: x + ParserState.value _ [] > x
+--   theorem sizeOf_opened_gt_popped_opened: x + ParserState.opened [] > x
+-- Otherwise we also need to make sure the following equations hold:
+--   theorem sizeOf_unknown_gt_opened: ParserState.unknown forest > ParserState.opened forest
+--   theorem sizeOf_value_value_gt_value:  ParserState.value _ ((ParseTree.mk v [])::nexts) > ParserState.value v nexts
+--   theorem sizeOf_opened_value_gt_value: ParserState.opened ((ParseTree.mk v [])::nexts) > ParserState.value v nexts
+--   theorem sizeOf_value_pair_gt_pair:  ParserState.value _ ((ParseTree.mk f [ParseTree.mk v []])::nexts) > ParserState.pair f v nexts
+--   theorem sizeOf_opened_pair_gt_pair: ParserState.opened ((ParseTree.mk f [ParseTree.mk v []])::nexts) > ParserState.pair f v nexts
+--   theorem sizeOf_pair_gt_value: ParserState.pair _ v nexts > ParserState.value v nexts
+--   theorem sizeOf_field_gt_opened: ParserState.field _ children > ParserState.opened children
+@[simp]
+noncomputable def ParserState.size (s: ParserState α): Nat :=
+  s.current.size + s.stack.size
+
+@[simp]
+noncomputable instance: SizeOf (ParserState α) where
+  sizeOf := ParserState.size
+
+def pop
+  [Monad m] [Debug m] [MonadExcept String m] [MonadStateOf (CurrentState α) m] [MonadStateOf (ParseStack α) m]:
+  m Unit := do
+  let top : Option (ParseForest α) <- Stack.popM?
+  match top with
+  | Option.some top' =>
+    set (CurrentState.opened top')
+    return ()
+  | Option.none =>
+    set (σ := CurrentState α) CurrentState.eof
+    return ()
 
 def nextNode
-  [Monad m] [Debug m] [MonadExcept String m] [MonadStateOf (TreeParser α) m]
+  [Monad m] [Debug m] [MonadExcept String m] [MonadStateOf (CurrentState α) m] [MonadStateOf (ParseStack α) m]
   (current: ParseTree α) (nexts: ParseForest α): m Hint := do
   match current with
   | ParseTree.mk v [] =>
-    Stack.setCurrent (ParserState.value v nexts)
+    set (CurrentState.value v nexts)
     return Hint.value
   | ParseTree.mk f [ParseTree.mk v []] =>
-    Stack.setCurrent (ParserState.pair f v nexts)
+    set (CurrentState.pair f v nexts)
     return Hint.field
   | ParseTree.mk f children =>
-    Stack.setCurrent (ParserState.opened nexts)
-    Stack.push (ParserState.field f children)
+    Stack.pushM nexts
+    set (CurrentState.field f children)
     return Hint.field
 
 def next
-  [Monad m] [Debug m] [MonadExcept String m] [MonadStateOf (TreeParser α) m]
+  [Monad m] [Debug m] [MonadExcept String m] [MonadState (CurrentState α) m] [MonadStateOf (CurrentState α) m] [MonadStateOf (ParseStack α) m]
   : m Hint := do
   Debug.debug "next"
-  let curr <- Stack.getCurrent
+  let curr <- get
   match curr with
-  | ParserState.unknown f =>
-    Stack.setCurrent (ParserState.opened f)
+  | CurrentState.unknown f =>
+    _ <- set (CurrentState.opened f)
     return Hint.enter
-  | ParserState.opened [] =>
-    let popped <- (TreeParser.pop (α := α))
-    if not popped then Stack.setCurrent (@ParserState.eof α)
+  | CurrentState.opened [] =>
+    pop (α := α)
     return Hint.leave
-  | ParserState.opened (t::ts) =>
+  | CurrentState.opened (t::ts) =>
     nextNode t ts
-  | ParserState.value _ [] =>
-    let popped <- (TreeParser.pop (α := α))
-    if not popped then Stack.setCurrent (@ParserState.eof α)
+  | CurrentState.value _ [] =>
+    pop (α := α)
     return Hint.leave
-  | ParserState.value _ (t::ts) =>
+  | CurrentState.value _ (t::ts) =>
     nextNode t ts
-  | ParserState.pair _ v nexts =>
-    Stack.setCurrent (ParserState.value v nexts)
+  | CurrentState.pair _ v nexts =>
+    _ <- set (CurrentState.value v nexts)
     return Hint.value
-  | ParserState.field _ children =>
-    Stack.setCurrent (ParserState.opened children)
+  | CurrentState.field _ children =>
+    _ <- set (CurrentState.opened children)
     return Hint.enter
-  | ParserState.eof =>
+  | CurrentState.eof =>
     return Hint.eof
 
 def skip
-  [Monad m] [Debug m] [MonadExcept String m] [MonadStateOf (TreeParser α) m]
+  [Monad m] [Debug m] [MonadExcept String m] [MonadState (CurrentState α) m] [MonadStateOf (CurrentState α) m] [MonadStateOf (ParseStack α) m]
   : m Unit := do
   Debug.debug "skip"
-  let curr <- Stack.getCurrent
+  let curr <- get
   match curr with
-  | ParserState.unknown _ =>
-    Stack.setCurrent (@ParserState.eof α)
-    return ()
-  | ParserState.opened _ =>
-    let popped <- (TreeParser.pop (α := α))
-    if not popped then Stack.setCurrent (@ParserState.eof α)
-    return ()
-  | ParserState.value _ _ =>
-    let popped: Bool <- (TreeParser.pop (α := α))
-    if not popped then Stack.setCurrent (@ParserState.eof α)
-    return ()
-  | ParserState.pair _ _ nexts =>
-    Stack.setCurrent (ParserState.opened nexts)
-    return ()
-  | ParserState.field _ _ =>
-    let popped: Bool <- (TreeParser.pop (α := α))
-    if not popped then Stack.setCurrent (@ParserState.eof α)
-    return ()
-  | ParserState.eof =>
-    return ()
+  | CurrentState.unknown _ => pop (α := α)
+  | CurrentState.opened _ => pop (α := α)
+  | CurrentState.value _ _ => pop (α := α)
+  | CurrentState.pair _ _ nexts => set (CurrentState.opened nexts)
+  | CurrentState.field _ _ => pop (α := α)
+  | CurrentState.eof => return ()
+  return ()
 
 def token
-  [Monad m] [Debug m] [MonadExcept String m] [MonadStateOf (TreeParser α) m]
+  [Monad m] [Debug m] [MonadExcept String m] [MonadStateOf (CurrentState α) m]
   : m α := do
   Debug.debug "token"
-  let curr <- Stack.getCurrent
+  let curr <- get
   match curr with
-  | ParserState.unknown _ =>
-    throw "unknown"
-  | ParserState.opened _ =>
-    throw "unknown"
-  | ParserState.value v _ =>
-    return v
-  | ParserState.pair f _ _ =>
-    return f
-  | ParserState.field f _ =>
-    return f
-  | ParserState.eof =>
-    throw "unknown"
+  | CurrentState.unknown _ => throw "unknown"
+  | CurrentState.opened _ => throw "unknown"
+  | CurrentState.value v _ => return v
+  | CurrentState.pair f _ _ => return f
+  | CurrentState.field f _ => return f
+  | CurrentState.eof => throw "unknown"
 
-instance [Monad m] [Debug m] [MonadExcept String m] [MonadStateOf (TreeParser α) m] : Parser m α where
+instance [Monad m] [Debug m] [MonadExcept String m] [MonadState (CurrentState α) m] [MonadStateOf (CurrentState α) m] [MonadStateOf (ParseStack α) m] : Parser m α where
   next := next (α := α)
   skip := skip (α := α)
   token := token
 
-def run (x: StateT (TreeParser α) (Except String) β) (t: ParseTree α): Except String β :=
-  StateT.run' x (TreeParser.mk t)
-
-instance : Debug (StateT (TreeParser α) (Except String)) where
+instance : Debug (StateT (ParserState α) (Except String)) where
   debug (_: String) := return ()
+
+abbrev TreeParser α β := StateT (ParserState α) (Except String) β
+
+def getStack [Monad m] [MonadStateOf (ParserState α) m] : m (ParseStack α) := do
+  let t: ParserState α <- MonadStateOf.get
+  return t.stack
+
+def setStack [Monad m] [MonadStateOf (ParserState α) m] (stack: ParseStack α) : m PUnit := do
+  let t: ParserState α <- MonadStateOf.get
+  MonadStateOf.set (ParserState.mk t.current stack)
+  return ()
+
+@[simp]
+instance instMonadStateOfParserStateMonadStateOfParseStack[Monad m] [MonadStateOf (ParserState α) m]: MonadStateOf (ParseStack α) m where
+  get : m (ParseStack α) := getStack
+  set (stack: ParseStack α) : m PUnit := setStack stack
+  modifyGet {β: Type} (f: ParseStack α → Prod β (ParseStack α)): m β := do
+    let t: ParserState α <- MonadStateOf.get
+    let (res, newstack) := f t.stack
+    MonadStateOf.set (ParserState.mk t.current newstack)
+    return res
+
+def getCurrent [Monad m] [MonadStateOf (ParserState α) m]: m (CurrentState α) := do
+  let t <- MonadState.get
+  return t.current
+
+def setCurrent [Monad m] [MonadStateOf (ParserState α) m] (current: CurrentState α) : m PUnit := do
+    let t <- MonadState.get
+    MonadStateOf.set (ParserState.mk current t.stack)
+    return ()
+
+def modifyGetCurrent [Monad m] [MonadStateOf (ParserState α) m] {β: Type} (f: CurrentState α → Prod β (CurrentState α)): m β := do
+    let t <- MonadState.get
+    let (res, newcurrent) := f t.current
+    MonadStateOf.set (ParserState.mk newcurrent t.stack)
+    return res
+
+@[simp]
+instance instMonadStateOfParserStateMonadStateOfCurrentState [Monad m] [MonadStateOf (ParserState α) m]: MonadStateOf (CurrentState α) m where
+  get : m (CurrentState α) := getCurrent
+  set (current: CurrentState α) : m PUnit := setCurrent current
+  modifyGet {β: Type} (f: CurrentState α → Prod β (CurrentState α)): m β := modifyGetCurrent f
+
+instance {α}: Parser (TreeParser α) α where
+  next := next
+  skip := skip
+  token := token
+
+def run' (x: TreeParser α β) (s: ParserState α): Except String β :=
+  StateT.run' x s
+
+def run (x: TreeParser α β) (s: ParserState α): Except String (β × (ParserState α)) :=
+  StateT.run x s
+
+def runTree (x: TreeParser α β) (t: ParseTree α): Except String β :=
+  StateT.run' x (ParserState.mk' t)
+
+theorem next_unknown_gt_opened:
+  run next (ParserState.mk (CurrentState.unknown children) stack) =
+  Except.ok (Hint.enter, ParserState.mk (CurrentState.opened children) stack) := by
+  simp [run, next, Debug.debug, getCurrent, setCurrent]
+  simp_monads
+
+theorem sizeOf_unknown_gt_opened:
+  sizeOf (ParserState.mk (CurrentState.unknown children) stack) >
+  sizeOf (ParserState.mk (CurrentState.opened children) stack) := by
+  simp
+
+theorem next_value_value_gt_value:
+  run next (ParserState.mk (CurrentState.value v' ((ParseTree.mk v [])::siblings)) stack) =
+  Except.ok (Hint.value, ParserState.mk (CurrentState.value v siblings) stack) := by
+  simp [run, next, nextNode, Debug.debug, getCurrent, setCurrent]
+  simp_monads
+
+theorem sizeOf_value_value_gt_value:
+  sizeOf (ParserState.mk (CurrentState.value v' ((ParseTree.mk v [])::siblings)) stack) >
+  sizeOf (ParserState.mk (CurrentState.value v siblings) stack) := by
+  simp
+
+theorem next_opened_value_gt_value:
+  run next (ParserState.mk (CurrentState.opened ((ParseTree.mk v [])::siblings)) stack) =
+  Except.ok (Hint.value, ParserState.mk (CurrentState.value v siblings) stack) := by
+  simp [run, next, nextNode, Debug.debug, getCurrent, setCurrent]
+  simp_monads
+
+theorem sizeOf_opened_value_gt_value:
+  sizeOf (ParserState.mk (CurrentState.opened ((ParseTree.mk v [])::siblings)) stack) >
+  sizeOf (ParserState.mk (CurrentState.value v siblings) stack) := by
+  simp
+
+theorem next_value_pair_gt_pair:
+  run next (ParserState.mk (CurrentState.value v' ((ParseTree.mk f [ParseTree.mk v []])::siblings)) stack) =
+  Except.ok (Hint.field, ParserState.mk (CurrentState.pair f v siblings) stack) := by
+  simp [run, next, nextNode, Debug.debug, getCurrent, setCurrent]
+  simp_monads
+
+theorem sizeOf_value_pair_gt_pair:
+  sizeOf (ParserState.mk (CurrentState.value v' ((ParseTree.mk f [ParseTree.mk v []])::siblings)) stack) >
+  sizeOf (ParserState.mk (CurrentState.pair f v siblings) stack) := by
+  simp +arith
+
+theorem next_opened_pair_gt_pair:
+  run next (ParserState.mk (CurrentState.opened ((ParseTree.mk f [ParseTree.mk v []])::siblings)) stack) =
+  Except.ok (Hint.field, ParserState.mk (CurrentState.pair f v siblings) stack) := by
+  simp [run, next, nextNode, Debug.debug, getCurrent, setCurrent]
+  simp_monads
+
+theorem sizeOf_opened_pair_gt_pair:
+  sizeOf (ParserState.mk (CurrentState.opened ((ParseTree.mk f [ParseTree.mk v []])::siblings)) stack) >
+  sizeOf (ParserState.mk (CurrentState.pair f v siblings) stack) := by
+  simp +arith
+
+theorem next_pair_gt_value:
+  run next (ParserState.mk (CurrentState.pair _k v siblings) stack) =
+  Except.ok (Hint.value, ParserState.mk (CurrentState.value v siblings) stack) := by
+  simp [run, next, nextNode, Debug.debug, getCurrent, setCurrent]
+  simp_monads
+
+theorem sizeOf_pair_gt_value:
+  sizeOf (ParserState.mk (CurrentState.pair _k v siblings) stack) >
+  sizeOf (ParserState.mk (CurrentState.value v siblings) stack) := by
+  simp
+
+theorem next_field_gt_opened:
+  run next (ParserState.mk (CurrentState.field f' children) stack) =
+  Except.ok (Hint.enter, ParserState.mk (CurrentState.opened children) stack) := by
+  simp [run, next, nextNode, Debug.debug, getCurrent, setCurrent]
+  simp_monads
+
+theorem sizeOf_field_gt_opened:
+  sizeOf (ParserState.mk (CurrentState.field f' children) stack) >
+  sizeOf (ParserState.mk (CurrentState.opened children) stack) := by
+  simp
+
+theorem next_opened_gt_push
+  {fchildren: ParseForest α}
+  -- if not a value and not a pair
+  (hc: (∃ v vchild vchildren, fchildren = [ParseTree.mk v (vchild::vchildren)])
+    \/ (∃ fchild1 fchild2 fchilds, fchildren = fchild1::fchild2::fchilds)):
+  run next (ParserState.mk ((CurrentState.opened ((ParseTree.mk f fchildren)::siblings))) stack) =
+  Except.ok (Hint.field, ParserState.mk (CurrentState.field f fchildren) (siblings::stack)) := by
+  cases hc with
+  | inl hc =>
+    obtain ⟨ v, vchild, vchildren, hc ⟩ := hc
+    rw [hc]
+    simp [run, next, nextNode, Debug.debug, getCurrent, setCurrent]
+    simp_monads
+    simp [Stack.pushM, getStack, setStack]
+    simp_monads
+  | inr hc =>
+    obtain ⟨ fchild1, fchild2, fchilds, hc ⟩ := hc
+    rw [hc]
+    simp [run, next, nextNode, Debug.debug, getCurrent, setCurrent]
+    simp_monads
+    simp [Stack.pushM, getStack, setStack]
+    simp_monads
+
+theorem sizeOf_opened_gt_push:
+  sizeOf (ParserState.mk ((CurrentState.opened ((ParseTree.mk f children)::siblings))) stack) >
+  sizeOf (ParserState.mk (CurrentState.field f children) (siblings::stack)) := by
+  simp +arith
+
+-- run next (ParserState.mk (CurrentState.value v' ((ParseTree.mk f [ParseTree.mk v []])::siblings)) stack) =
+-- run next (ParserState.mk (CurrentState.value v' ((ParseTree.mk v [])::siblings)) stack) =
+theorem next_value_gt_push
+  {fchildren: ParseForest α}
+  -- if not a value and not a pair
+  (hc: (∃ v vchild vchildren, fchildren = [ParseTree.mk v (vchild::vchildren)])
+    \/ (∃ fchild1 fchild2 fchilds, fchildren = fchild1::fchild2::fchilds)):
+  run next (ParserState.mk (CurrentState.value v ((ParseTree.mk f fchildren)::fsiblings)) stack) =
+  Except.ok (Hint.field, ParserState.mk (CurrentState.field f fchildren) (fsiblings::stack)) := by
+  cases hc with
+  | inl hc =>
+    obtain ⟨ v, vchild, vchildren, hc ⟩ := hc
+    rw [hc]
+    simp [run, next, nextNode, Debug.debug, getCurrent, setCurrent]
+    simp_monads
+    simp [Stack.pushM, getStack, setStack]
+    simp_monads
+  | inr hc =>
+    obtain ⟨ fchild1, fchild2, fchilds, hc ⟩ := hc
+    rw [hc]
+    simp [run, next, nextNode, Debug.debug, getCurrent, setCurrent]
+    simp_monads
+    simp [Stack.pushM, getStack, setStack]
+    simp_monads
+
+theorem sizeOf_value_gt_push:
+  sizeOf (ParserState.mk ((CurrentState.value v ((ParseTree.mk f children)::siblings))) stack) >
+  sizeOf (ParserState.mk (CurrentState.field f children) (siblings::stack)) := by
+  simp +arith
+
+theorem next_value_gt_popped_value_eof {α: Type} (v: α):
+  run next (ParserState.mk (α := α) (CurrentState.value v []) []) =
+  Except.ok (Hint.leave, ParserState.mk (α := α) CurrentState.eof []) := by
+  simp [run, next, nextNode, Debug.debug, getCurrent, setCurrent]
+  simp_monads
+  simp [pop, Stack.popM?, getStack]
+  simp_monads
+
+theorem sizeOf_value_gt_popped_value_eof {α: Type}:
+  sizeOf (ParserState.mk (CurrentState.value _v []) []) >
+  sizeOf (ParserState.mk (α := α) CurrentState.eof []) := by
+  simp
+
+theorem next_value_gt_popped_value_more:
+  run next (ParserState.mk (CurrentState.value _v []) (elem::stack)) =
+  Except.ok (Hint.leave, ParserState.mk (CurrentState.opened elem) stack) := by
+  simp [run, next, nextNode, Debug.debug, getCurrent, setCurrent]
+  simp_monads
+  simp [pop, Stack.popM?, getStack, setStack]
+  simp_monads
+
+theorem sizeOf_value_gt_popped_value_more:
+  sizeOf (ParserState.mk (CurrentState.value _v []) (elem::stack)) >
+  sizeOf (ParserState.mk (CurrentState.opened elem) stack) := by
+  simp +arith
+
+theorem next_opened_gt_popped_opened_eof {α: Type}:
+  run next (ParserState.mk (α := α) (CurrentState.opened []) []) =
+  Except.ok (Hint.leave, ParserState.mk (α := α) CurrentState.eof []) := by
+  simp [run, next, nextNode, Debug.debug, getCurrent, setCurrent]
+  simp_monads
+  simp [pop, Stack.popM?, getStack, setStack]
+  simp_monads
+
+theorem sizeOf_opened_gt_popped_opened_eof {α: Type}:
+  sizeOf (ParserState.mk (α := α) (CurrentState.opened []) []) >
+  sizeOf (ParserState.mk (α := α) CurrentState.eof []) := by
+  simp
+
+theorem next_opened_gt_popped_opened_more:
+  run next (ParserState.mk (CurrentState.opened []) (elem::stack)) =
+  Except.ok (Hint.leave, ParserState.mk (CurrentState.opened elem) stack) := by
+  simp [run, next, nextNode, Debug.debug, getCurrent, setCurrent]
+  simp_monads
+  simp [pop, Stack.popM?, getStack, setStack]
+  simp_monads
+
+theorem sizeOf_opened_gt_popped_opened_more:
+  sizeOf (ParserState.mk (CurrentState.opened []) (elem::stack)) >
+  sizeOf (ParserState.mk (CurrentState.opened elem) stack) := by
+  simp +arith
+
+theorem next_eof_gt_eof:
+  run next (ParserState.mk CurrentState.eof stack) =
+  Except.ok (Hint.eof, ParserState.mk CurrentState.eof stack) := by
+  simp [run, next, Debug.debug, getCurrent]
+  simp_monads
 
 open Parser (walk Action)
 open TokenTree (node)
 
-#guard run
+#guard run'
+  next
+  (ParserState.mk (CurrentState.unknown [ParseTree.mk 0 []]) [])
+  = Except.ok Hint.enter
+
+#guard runTree
   (walk [Action.next, Action.next, Action.next])
   (node "a" []) =
   Except.ok ["{", "V", "}"]
 
-#guard run
+#guard runTree
   (walk [Action.next, Action.next, Action.next, Action.next, Action.next, Action.next, Action.next, Action.next])
   (node "a" [node "b" [], node "c" [node "d" []]]) =
   Except.ok ["{", "F", "{", "V", "F", "V", "}", "}"]
 
 -- walk next just two
-#guard run
+#guard runTree
   (walk [Action.next, Action.next])
   (node "a" [node "b" [], node "c" [node "d" []]])
   = Except.ok ["{", "F"]
 
 -- walk next to end
-#guard run
+#guard runTree
   (walk [Action.next, Action.next, Action.next, Action.next, Action.next, Action.next, Action.next, Action.next, Action.next])
   (node "a" [node "b" [], node "c" [node "d" []]])
   = Except.ok ["{", "F", "{", "V", "F", "V", "}", "}", "$"]
 
 -- walk next to end and tokenize all
-#guard run
+#guard runTree
   (walk [Action.next, Action.next, Action.token, Action.next, Action.next, Action.token, Action.next, Action.token, Action.next, Action.token, Action.next, Action.next, Action.next])
   (node "a" [node "b" [], node "c" [node "d" []]])
   = Except.ok ["{", "F", "a", "{", "V", "b", "F", "c", "V", "d", "}", "}", "$"]
 
 -- walk next to end and tokenize all
-#guard run
+#guard runTree
   (walk [Action.next, Action.next, Action.token, Action.next, Action.next, Action.token, Action.next, Action.token, Action.next, Action.token, Action.next, Action.next, Action.next])
   (node "a" [node "b" [], node "c" [node "d" []]])
   = Except.ok ["{", "F", "a", "{", "V", "b", "F", "c", "V", "d", "}", "}", "$"]
 
 -- walk skip
-#guard run
+#guard runTree
   (walk [Action.skip, Action.next])
   (node "a" [node "b" [], node "c" [node "d" []]]) =
   Except.ok ["$"]
 
 -- walk next skip
-#guard run
+#guard runTree
   (walk [Action.next, Action.skip, Action.next])
   (node "a" [node "b" [], node "c" [node "d" []]]) =
   Except.ok ["{", "$"]
 
 -- walk next next skip
-#guard run
+#guard runTree
   (walk [Action.next, Action.next, Action.skip, Action.next, Action.next])
   (node "a" [node "b" [], node "c" [node "d" []]]) =
   Except.ok ["{", "F", "}", "$"]
 
 -- walk next next token skip
-#guard run
+#guard runTree
   (walk [Action.next, Action.next, Action.token, Action.skip, Action.next, Action.next])
   (node "a" [node "b" [], node "c" [node "d" []]]) =
   Except.ok ["{", "F", "a", "}", "$"]
 
 -- walk next next token next skip
-#guard run
+#guard runTree
   (walk [Action.next, Action.next, Action.token, Action.next, Action.skip, Action.next, Action.next])
   (node "a" [node "b" [], node "c" [node "d" []]]) =
   Except.ok ["{", "F", "a", "{", "}", "$"]
 
 -- walk next next token next next token skip
-#guard run
+#guard runTree
   (walk [Action.next, Action.next, Action.token, Action.next, Action.next, Action.token, Action.skip, Action.next, Action.next])
   (node "a" [node "b" [], node "c" [node "d" []]]) =
   Except.ok ["{", "F", "a", "{", "V", "b", "}", "$"]
 
 -- walk next next token next next token next token skip
-#guard run
+#guard runTree
   (walk [Action.next, Action.next, Action.token, Action.next, Action.next, Action.token, Action.next, Action.token, Action.skip, Action.next, Action.next, Action.next])
   (node "a" [node "b" [], node "c" [node "d" []]]) =
   Except.ok ["{", "F", "a", "{", "V", "b", "F", "c", "}", "}", "$"]
+
+theorem next_decreases_stack_size
+  {hint: Hint}
+  {thisParserState nextParserState: ParserState α}
+  (hneof: hint ≠ Hint.eof)
+  (h: Except.ok (hint, nextParserState) = run next thisParserState):
+  sizeOf nextParserState < sizeOf thisParserState := by
+  have h' := Eq.symm h
+  clear h
+  have h := congrArg (Except.map (fun x => x.snd)) h'
+  simp [Except.map] at h
+  cases thisParserState with
+  | mk thisCurrent thisStack =>
+  cases thisCurrent with
+  | unknown xs =>
+    rw [next_unknown_gt_opened] at h
+    simp at h
+    rw [<- h]
+    exact sizeOf_unknown_gt_opened
+  | opened xs =>
+    cases xs with
+    | nil =>
+      cases thisStack with
+      | nil =>
+        rw [next_opened_gt_popped_opened_eof] at h
+        simp at h
+        rw [<- h]
+        exact sizeOf_opened_gt_popped_opened_eof
+      | cons s' ss' =>
+        rw [next_opened_gt_popped_opened_more] at h
+        simp at h
+        rw [<- h]
+        exact sizeOf_opened_gt_popped_opened_more
+    | cons tree fsiblings =>
+      cases tree with
+      | mk f v =>
+        cases v with
+        | nil =>
+          -- is value
+          rw [next_opened_value_gt_value] at h
+          simp at h
+          rw [<- h]
+          exact sizeOf_opened_value_gt_value
+        | cons v vsiblings =>
+          -- is pair or field
+          cases v with
+          | mk v vchildren =>
+            cases vchildren with
+            | nil =>
+              cases vsiblings with
+              | nil =>
+                -- is pair
+                rw [next_opened_pair_gt_pair] at h
+                simp at h
+                rw [<- h]
+                exact sizeOf_opened_pair_gt_pair
+              | cons vsibling vsiblings =>
+                -- is field
+                rw [next_opened_gt_push] at h
+                simp at h
+                rw [<- h]
+                apply sizeOf_opened_gt_push
+                right
+                exists ParseTree.mk v []
+                exists vsibling
+                exists vsiblings
+            | cons vchild vchildren =>
+              -- if field
+              rw [next_opened_gt_push] at h
+              simp at h
+              rw [<- h]
+              apply sizeOf_opened_gt_push
+              cases vsiblings with
+              | nil =>
+                left
+                exists v
+                exists vchild
+                exists vchildren
+              | cons vsibling vsiblings =>
+                right
+                exists ParseTree.mk v (vchild :: vchildren)
+                exists vsibling
+                exists vsiblings
+  | value x xs =>
+    cases xs with
+    | nil =>
+      cases thisStack with
+      | nil =>
+        rw [next_value_gt_popped_value_eof] at h
+        simp at h
+        rw [<- h]
+        exact sizeOf_value_gt_popped_value_eof
+      | cons s' ss' =>
+        rw [next_value_gt_popped_value_more] at h
+        simp at h
+        rw [<- h]
+        exact sizeOf_value_gt_popped_value_more
+    | cons tree fsiblings =>
+      cases tree with
+      | mk f v =>
+        cases v with
+        | nil =>
+          -- is value
+          rw [next_value_value_gt_value] at h
+          simp at h
+          rw [<- h]
+          exact sizeOf_opened_value_gt_value
+        | cons v vsiblings =>
+          -- is pair or field
+          cases v with
+          | mk v vchildren =>
+            cases vchildren with
+            | nil =>
+              cases vsiblings with
+              | nil =>
+                -- is pair
+                rw [next_value_pair_gt_pair] at h
+                simp at h
+                rw [<- h]
+                exact sizeOf_opened_pair_gt_pair
+              | cons vsibling vsiblings =>
+                -- is field
+                rw [next_value_gt_push] at h
+                simp at h
+                rw [<- h]
+                apply sizeOf_opened_gt_push
+                right
+                exists ParseTree.mk v []
+                exists vsibling
+                exists vsiblings
+            | cons vchild vchildren =>
+              -- if field
+              rw [next_value_gt_push] at h
+              simp at h
+              rw [<- h]
+              apply sizeOf_opened_gt_push
+              cases vsiblings with
+              | nil =>
+                left
+                exists v
+                exists vchild
+                exists vchildren
+              | cons vsibling vsiblings =>
+                right
+                exists ParseTree.mk v (vchild :: vchildren)
+                exists vsibling
+                exists vsiblings
+  | pair f v xs =>
+    rw [next_pair_gt_value] at h
+    simp at h
+    rw [<- h]
+    exact sizeOf_pair_gt_value
+  | field f xs =>
+    rw [next_field_gt_opened] at h
+    simp at h
+    rw [<- h]
+    exact sizeOf_field_gt_opened
+  | eof =>
+    rw [next_eof_gt_eof] at h'
+    simp at h'
+    obtain ⟨heof, _⟩ := h'
+    rw [<- heof] at hneof
+    contradiction
