Validator/Validator/Inst/TreeParserIO.lean
@@ -11,13 +11,13 @@ import Validator.Validator.ValidateM
 namespace TreeParserIO
 
 structure State (α: Type) [DecidableEq α] [Hashable α] where
-  parser: TreeParser.TreeParser α
+  parser: TreeParser.ParserState α
   enter: MemEnter.EnterMap α
   leave: MemLeave.LeaveMap α
 
 abbrev Impl α [DecidableEq α] [Hashable α] β := StateT (State α) (EIO String) β
 
-def Impl.mk [DecidableEq α] [Hashable α] (p: TreeParser.TreeParser α): State α :=
+def Impl.mk [DecidableEq α] [Hashable α] (p: TreeParser.ParserState α): State α :=
   State.mk p MemEnter.EnterMap.mk MemLeave.LeaveMap.mk
 
 def EIO.println [ToString α] (x: α): EIO String Unit :=
@@ -26,15 +26,15 @@ def EIO.println [ToString α] (x: α): EIO String Unit :=
 instance [DecidableEq α] [Hashable α] : Debug (Impl α) where
   debug (line: String) := StateT.lift (EIO.println line)
 
-instance [DecidableEq α] [Hashable α]: MonadStateOf (TreeParser.TreeParser α) (Impl α) where
-  get : Impl α (TreeParser.TreeParser α) := do
+instance [DecidableEq α] [Hashable α]: MonadStateOf (TreeParser.ParserState α) (Impl α) where
+  get : Impl α (TreeParser.ParserState α) := do
     let s <- StateT.get
     return s.parser
-  set : TreeParser.TreeParser α → Impl α PUnit :=
+  set : TreeParser.ParserState α → Impl α PUnit :=
     fun parser => do
       let s <- StateT.get
       set (State.mk parser s.enter s.leave)
-  modifyGet {β: Type}: (TreeParser.TreeParser α → Prod β (TreeParser.TreeParser α)) → Impl α β :=
+  modifyGet {β: Type}: (TreeParser.ParserState α → Prod β (TreeParser.ParserState α)) → Impl α β :=
     fun f => do
       let s <- StateT.get
       let (res, parser) := f s.parser
@@ -47,7 +47,7 @@ instance
   [Monad (Impl α)] -- EStateM is monad
   [Debug (Impl α)] -- Debug instance is declared above
   [MonadExcept String (Impl α)] -- EStateM String is MonadExcept String
-  [MonadStateOf (TreeParser.TreeParser α) (Impl α)] -- MonadStateOf ParseTree.TreeParser is declared above
+  [MonadStateOf (TreeParser.ParserState α) (Impl α)] -- MonadStateOf ParseTree.TreeParser is declared above
   : Parser (Impl α) α where -- This should just follow, but apparently we need to spell it out
   next := Parser.next
   skip := Parser.skip
@@ -83,4 +83,4 @@ instance [DecidableEq α] [Hashable α]: ValidateM (Impl α) α where
   -- all instances have been created, so no implementations are required here
 
 def run' [DecidableEq α] [Hashable α] (f: Impl α β) (t: ParseTree α): EIO String β :=
-  StateT.run' f (Impl.mk (TreeParser.TreeParser.mk t))
+  StateT.run' f (Impl.mk (TreeParser.ParserState.mk' t))
