Validator.lean
@@ -1,4 +1,5 @@
 import Validator.Std.Linter.DetectClassical
+import Validator.Std.Ltac
 import Validator.Std.Debug
 import Validator.Std.Except
 
