Validator/Parser/ParseTreeIterator.lean
@@ -1,0 +1,225 @@
+import Init.Data.Iterators
+
+import Validator.Parser.Hint
+import Validator.Parser.ParseTree
+import Validator.Parser.TreeParser
+
+structure ParseTreeIterator (α : Type) where
+  state : TreeParser.ParserState α
+
+def ParseForest.iterM {α : Type} (forest : ParseForest α) (m : Type → Type w') [Pure m] :
+  Std.Iterators.IterM (α := ParseTreeIterator α) m α :=
+    Std.Iterators.toIterM { state := TreeParser.ParserState.mks forest } m α
+
+def PlausibleIterStep (IsPlausibleStep : Std.Iterators.IterStep α β → Prop) := Subtype IsPlausibleStep
+class Iterator (α : Type w) (m : Type w → Type w') (β : outParam (Type w)) where
+  IsPlausibleStep : Std.Iterators.IterM (α := α) m β → Std.Iterators.IterStep (Std.Iterators.IterM (α := α) m β) β → Prop
+  step : (it : Std.Iterators.IterM (α := α) m β) → m (PlausibleIterStep (IsPlausibleStep it))
+
+instance {α : Type} [Pure m] : Std.Iterators.Iterator (ParseTreeIterator α) m Hint where
+  IsPlausibleStep
+    (currentState: @Std.IterM (ParseTreeIterator α) m Hint)
+    (iterStep: Std.Iterators.IterStep (@Std.Iterators.IterM (ParseTreeIterator α) m Hint) Hint): Prop :=
+    match iterStep with
+    | .skip _ => False
+    | .done => currentState.internalState.state.current = TreeParser.CurrentState.eof
+    | .yield nextState nextHint =>
+      nextHint ≠ Hint.eof /\
+      Except.ok (nextHint, nextState.internalState.state) = TreeParser.run (TreeParser.next (α := α)) currentState.internalState.state
+  step (it: @Std.IterM (ParseTreeIterator α) m Hint)
+    -- def PlausibleIterStep
+    --   (IsPlausibleStep : Std.Iterators.IterStep (@Std.Iterators.IterM (ParseTreeIterator α) m Hint) Hint → Prop) :=
+    --   Subtype IsPlausibleStep
+    -- : m (PlausibleIterStep (IsPlausibleStep it))
+    := by
+      let ⟨ ⟨ current, stack ⟩ ⟩ := it
+      cases current with
+      | unknown children =>
+        refine (pure ⟨ Std.Iterators.IterStep.yield ⟨ParseTreeIterator.mk ?_⟩ ?_, ?_ ⟩ )
+        · exact (TreeParser.ParserState.mk (TreeParser.CurrentState.opened children) stack)
+        · exact Hint.enter
+        · simp
+          rw [<- TreeParser.next_unknown_gt_opened]
+      | field f children =>
+        refine (pure ⟨ Std.Iterators.IterStep.yield ⟨ParseTreeIterator.mk ?_⟩ ?_, ?_ ⟩ )
+        · exact (TreeParser.ParserState.mk (TreeParser.CurrentState.opened children) stack)
+        · exact Hint.enter
+        · simp
+          rw [<- TreeParser.next_field_gt_opened]
+      | pair f v children =>
+        refine (pure ⟨ Std.Iterators.IterStep.yield ⟨ParseTreeIterator.mk ?_⟩ ?_, ?_ ⟩ )
+        · exact (TreeParser.ParserState.mk (TreeParser.CurrentState.value v children) stack)
+        · exact Hint.value
+        · simp
+          rw [<- TreeParser.next_pair_gt_value]
+      | opened children =>
+        cases children with
+        | nil =>
+          cases stack with
+          | nil =>
+            refine (pure ⟨ Std.Iterators.IterStep.yield ⟨ParseTreeIterator.mk ?_⟩ ?_, ?_ ⟩ )
+            · exact (TreeParser.ParserState.mk TreeParser.CurrentState.eof [])
+            · exact Hint.leave
+            · simp
+              rw [TreeParser.next_opened_gt_popped_opened_eof]
+          | cons s ss =>
+            refine (pure ⟨ Std.Iterators.IterStep.yield ⟨ParseTreeIterator.mk ?_⟩ ?_, ?_ ⟩ )
+            · exact (TreeParser.ParserState.mk (TreeParser.CurrentState.opened s) ss)
+            · exact Hint.leave
+            · simp
+              rw [TreeParser.next_opened_gt_popped_opened_more]
+        | cons child siblings =>
+          cases child with
+          | mk f fchildren =>
+            cases fchildren with
+            | nil =>
+              refine (pure ⟨ Std.Iterators.IterStep.yield ⟨ParseTreeIterator.mk ?_⟩ ?_, ?_ ⟩ )
+              · exact (TreeParser.ParserState.mk (TreeParser.CurrentState.value f siblings) stack)
+              · exact Hint.value
+              · simp
+                rw [TreeParser.next_opened_value_gt_value]
+            | cons fchild1 fchildren =>
+              cases fchildren with
+              | nil =>
+                cases fchild1 with
+                | mk v vchildren =>
+                cases vchildren with
+                | nil =>
+                  refine (pure ⟨ Std.Iterators.IterStep.yield ⟨ParseTreeIterator.mk ?_⟩ ?_, ?_ ⟩ )
+                  · exact (TreeParser.ParserState.mk (TreeParser.CurrentState.pair f v siblings) stack)
+                  · exact Hint.field
+                  · simp
+                    rw [TreeParser.next_opened_pair_gt_pair]
+                | cons vchild vchildren =>
+                  refine (pure ⟨ Std.Iterators.IterStep.yield ⟨ParseTreeIterator.mk ?_⟩ ?_, ?_ ⟩ )
+                  · exact (TreeParser.ParserState.mk (TreeParser.CurrentState.field f [ParseTree.mk v (vchild::vchildren)]) (siblings::stack))
+                  · exact Hint.field
+                  · simp
+                    rw [TreeParser.next_opened_gt_push]
+                    left
+                    exists v
+                    exists vchild
+                    exists vchildren
+              | cons fchild2 fchildren =>
+                refine (pure ⟨ Std.Iterators.IterStep.yield ⟨ParseTreeIterator.mk ?_⟩ ?_, ?_ ⟩ )
+                · exact (TreeParser.ParserState.mk (TreeParser.CurrentState.field f (fchild1::fchild2::fchildren)) (siblings::stack))
+                · exact Hint.field
+                · simp
+                  rw [TreeParser.next_opened_gt_push]
+                  right
+                  exists fchild1
+                  exists fchild2
+                  exists fchildren
+      | value v children =>
+        cases children with
+        | nil =>
+          cases stack with
+          | nil =>
+            refine (pure ⟨ Std.Iterators.IterStep.yield ⟨ParseTreeIterator.mk ?_⟩ ?_, ?_ ⟩ )
+            · exact (TreeParser.ParserState.mk TreeParser.CurrentState.eof [])
+            · exact Hint.leave
+            · simp
+              rw [TreeParser.next_value_gt_popped_value_eof]
+          | cons s ss =>
+            refine (pure ⟨ Std.Iterators.IterStep.yield ⟨ParseTreeIterator.mk ?_⟩ ?_, ?_ ⟩ )
+            · exact (TreeParser.ParserState.mk (TreeParser.CurrentState.opened s) ss)
+            · exact Hint.leave
+            · simp
+              rw [TreeParser.next_value_gt_popped_value_more]
+        | cons child siblings =>
+          cases child with
+          | mk f fchildren =>
+            cases fchildren with
+            | nil =>
+              refine (pure ⟨ Std.Iterators.IterStep.yield ⟨ParseTreeIterator.mk ?_⟩ ?_, ?_ ⟩ )
+              · exact (TreeParser.ParserState.mk (TreeParser.CurrentState.value f siblings) stack)
+              · exact Hint.value
+              · simp
+                rw [TreeParser.next_value_value_gt_value]
+            | cons fchild1 fchildren =>
+              cases fchildren with
+              | nil =>
+                cases fchild1 with
+                | mk v vchildren =>
+                cases vchildren with
+                | nil =>
+                  refine (pure ⟨ Std.Iterators.IterStep.yield ⟨ParseTreeIterator.mk ?_⟩ ?_, ?_ ⟩ )
+                  · exact (TreeParser.ParserState.mk (TreeParser.CurrentState.pair f v siblings) stack)
+                  · exact Hint.field
+                  · simp
+                    rw [TreeParser.next_value_pair_gt_pair]
+                | cons vchild vchildren =>
+                  refine (pure ⟨ Std.Iterators.IterStep.yield ⟨ParseTreeIterator.mk ?_⟩ ?_, ?_ ⟩ )
+                  · exact (TreeParser.ParserState.mk (TreeParser.CurrentState.field f [ParseTree.mk v (vchild::vchildren)]) (siblings::stack))
+                  · exact Hint.field
+                  · simp
+                    rw [TreeParser.next_value_gt_push]
+                    left
+                    exists v
+                    exists vchild
+                    exists vchildren
+              | cons fchild2 fchildren =>
+                refine (pure ⟨ Std.Iterators.IterStep.yield ⟨ParseTreeIterator.mk ?_⟩ ?_, ?_ ⟩ )
+                · exact (TreeParser.ParserState.mk (TreeParser.CurrentState.field f (fchild1::fchild2::fchildren)) (siblings::stack))
+                · exact Hint.field
+                · simp
+                  rw [TreeParser.next_value_gt_push]
+                  right
+                  exists fchild1
+                  exists fchild2
+                  exists fchildren
+      | eof =>
+        refine (pure ⟨ Std.Iterators.IterStep.done, ?_ ⟩ )
+        simp
+
+private def ParseTreeIterator.finitenessRelation [Pure m] :
+    Std.Iterators.FinitenessRelation (ParseTreeIterator α) m where
+  rel := InvImage WellFoundedRelation.rel (ParseTreeIterator.state ∘ Std.Iterators.IterM.internalState)
+  wf := InvImage.wf _ WellFoundedRelation.wf
+  subrelation {it it'} h := by
+    clean_wf
+    simp only [Function.comp]
+    obtain ⟨step, h, h'⟩ := h
+    cases step with
+    | skip =>
+      simp_all [Std.Iterators.IterStep.successor, Std.Iterators.IterM.IsPlausibleStep, Std.Iterators.Iterator.IsPlausibleStep]
+    | done =>
+      simp_all [Std.Iterators.IterStep.successor]
+    | yield =>
+      rename_i hint
+      simp only [Std.Iterators.IterM.IsPlausibleStep, Std.Iterators.Iterator.IsPlausibleStep] at h'
+      simp [Std.Iterators.IterStep.successor] at h
+      rw [h] at h'
+      obtain ⟨ hneof, h' ⟩ := h'
+      exact TreeParser.next_decreases_stack_size hneof h'
+
+instance [Pure m] : Std.Iterators.Finite (ParseTreeIterator α) m :=
+  Std.Iterators.Finite.of_finitenessRelation ParseTreeIterator.finitenessRelation
+
+@[always_inline, inline]
+instance {α : Type} [Monad m] {n : Type → Type w''} [Monad n] :
+    Std.Iterators.IteratorCollect (ParseTreeIterator α) m n :=
+  .defaultImplementation
+
+@[always_inline, inline]
+instance {α : Type} [Monad m] {n : Type → Type w''} [Monad n] :
+    Std.Iterators.IteratorCollectPartial (ParseTreeIterator α) m n :=
+  .defaultImplementation
+
+@[always_inline, inline]
+instance {α : Type} [Monad m] {n : Type → Type x'} [Monad n] :
+    Std.Iterators.IteratorLoop (ParseTreeIterator α) m n :=
+  .defaultImplementation
+
+@[always_inline, inline]
+instance {α : Type} [Monad m] {n : Type → Type x'} [Monad n] :
+    Std.Iterators.IteratorLoopPartial (ParseTreeIterator α) m n :=
+  .defaultImplementation
+
+@[always_inline, inline]
+instance {α : Type} [Monad m] : Std.Iterators.IteratorSize (ParseTreeIterator α) m :=
+  .defaultImplementation
+
+@[always_inline, inline]
+instance {α : Type} [Monad m] : Std.Iterators.IteratorSizePartial (ParseTreeIterator α) m :=
+  .defaultImplementation
