Validator/Validator/Inst/TreeParserM.lean
@@ -4,7 +4,7 @@ import Validator.Validator.ValidateM
 
 namespace TreeParserM
 
-abbrev Impl α β := EStateM String (TreeParser.TreeParser α) β
+abbrev Impl α β := EStateM String (TreeParser.ParserState α) β
 
 instance : Debug (Impl α) where
   debug (_line: String) := return ()
@@ -13,7 +13,7 @@ instance
   [Monad (Impl α)] -- EStateM is monad
   [Debug (Impl α)] -- Debug instance is declared above
   [MonadExcept String (Impl α)] -- EStateM String is MonadExcept String
-  [MonadStateOf (TreeParser.TreeParser α) (Impl α)] -- EStateM ε ParseTree.TreeParser is a MonadStateOf ParseTree.TreeParser
+  [MonadStateOf (TreeParser.ParserState α) (Impl α)] -- EStateM ε ParseTree.TreeParser is a MonadStateOf ParseTree.TreeParser
   : Parser (Impl α) α where -- This should just follow, but apparently we need to spell it out
   next := Parser.next
   skip := Parser.skip
@@ -29,6 +29,6 @@ instance [DecidableEq α]: ValidateM (Impl α) α where
   -- all instances have been created, so no implementations are required here
 
 def run' (x: Impl α β) (t: ParseTree α): Except String β :=
-  match EStateM.run x (TreeParser.TreeParser.mk t) with
+  match EStateM.run x (TreeParser.ParserState.mk' t) with
   | EStateM.Result.ok k _ => Except.ok k
   | EStateM.Result.error err _ => Except.error err
