learnings/simp_arith.md
@@ -1,0 +1,27 @@
+# simp_arith
+
+`simp +arith` is a tactic that does simplification and includes simplifying arithmetic.
+This means you can replace `simp ; omega` with `simp +airth`.
+This doesn't seem that useful, but it really shines when you add extra definitions for simp to include.
+
+```lean
+def add1 x := x + 1
+
+example: (add1 x) + 1 = add1 1 + x := by
+  simp [add1]
+  omega
+
+example: (add1 x) + 1 = add1 1 + x := by
+  simp +airth [add1]
+```
+
+This also works if `add1` was included in the `simp` library:
+
+
+```lean
+@[simp]
+def add1' x := x + 1
+
+example: (add1' x) + 1 = add1' 1 + x := by
+  simp +arith
+```
